

1. ให้ $u = (4, 0, -3, 5)$, $v = (0, 2, 5, 4)$

จงหา (a) $u - v$

(b) $2(u + 3v)$

(c) $2v - u$

(a) $= (4 - 0, 0 - 2, (-3) - 5, 5 - 4)$
 $= (4, -2, -8, 1)$ ~~\neq~~

(b) $= 2((4, 0, -3, 5) + (3)(0, 2, 5, 4))$
 $= 2((4, 0, -3, 5) + (0, 6, 15, 12))$
 $= 2(4, 6, 12, 17)$
 $= (8, 12, 24, 34)$ ~~\neq~~

(c) $= 2((2)(0, 2, 5, 4) - (4, 0, -3, 5))$
 $= (0, 4, 10, 8) - (4, 0, -3, 5)$
 $= (-4, 4, 13, 3)$ ~~\neq~~

$$2. \text{ให้ } u = (1, -1, 0, 1) \text{ และ } v = (0, 2, 3, -1)$$

$$\text{หา } w \text{ ที่ } u \perp w \text{ และ } v \perp w \text{ โดย } 2w = u - 3v$$

$$2w = (1, -1, 0, 1) - (0, 6, 9, -3)$$

$$2w = (1, -7, -9, 4)$$

$$w = \frac{1}{2} (1, -7, -9, 4)$$

$$w = \left(\frac{1}{2}, -\frac{7}{2}, -\frac{9}{2}, 2 \right)$$

$$\|w\| = \sqrt{\left(\frac{1}{2}\right)^2 + \left(-\frac{7}{2}\right)^2 + \left(-\frac{9}{2}\right)^2 + 2^2}$$

$$= \sqrt{\frac{1}{4} + \frac{49}{4} + \frac{81}{4} + 4}$$

$$= \sqrt{\frac{1 + 49 + 81 + (4)(4)}{4}}$$

$$\|w\| = \sqrt{\frac{147}{4}}$$

3. ให้ $u = (-1, 1, -2)$ และ $v = (1, -3, -2)$

จงหา (a) $u \cdot v$

(b) $u \cdot u$

(c) $\|u\|^2$

$$\begin{aligned} \text{(a)} \quad u \cdot v &= (-1)(1) + (1)(-3) + (-2)(-2) \\ &= -1 - 3 + 4 \\ &= 0 \quad \# \end{aligned}$$

$$\begin{aligned} \text{(b)} \quad u \cdot u &= (-1)(-1) + (1)(1) + (-2)(-2) \\ &= 1 + 1 + 4 \\ &= 6 \quad \# \end{aligned}$$

$$\begin{aligned} \text{(c)} \quad \|u\|^2 &= \sqrt{(-1)^2 + (1)^2 + (-2)^2}^2 \\ &= \sqrt{6}^2 \\ \|u\|^2 &= 6 \quad \# \end{aligned}$$

4. ให้ $u = (3, 1), v = (-2, 4)$

จงหาขนาด θ ระหว่างเวกเตอร์

$$\frac{u \cdot v}{\|u\| \|v\|} = \frac{(3)(-2) + (1)(4)}{\sqrt{3^2 + 1^2} \sqrt{(-2)^2 + (4)^2}}$$

$$= \frac{-2}{\sqrt{20}}$$

$$= \frac{-2}{10\sqrt{2}}$$

$$= \frac{-2\sqrt{2}}{20}$$

$$= \frac{-\sqrt{2}}{10}$$

$$= 40^\circ$$

5. ให้ $u = (12, -3, 1), v = (-2, 5, 1)$

จงหาผลคูณของ $u \times v$ / $u \cdot v$ = 1 แสดงว่า u และ v ตั้งฉากกัน หรือหาผลคูณ $u \cdot v = V$

$$u \times v = \begin{vmatrix} i & j & k \\ 12 & -3 & 1 \\ -2 & 5 & 1 \end{vmatrix}$$

$$= \begin{vmatrix} -3 & 1 \\ 5 & 1 \end{vmatrix} i - \begin{vmatrix} 12 & 1 \\ -2 & 1 \end{vmatrix} j + \begin{vmatrix} 12 & -3 \\ -2 & 5 \end{vmatrix} k$$

$$= -8i - 14j + 54k$$

$$u \cdot (u \times v) = 12(-8) + (-3)(-14) + (1)(54)$$

$$= 0 \text{ ตั้งฉาก } \#$$

$$v \cdot (u \times v) = (-2)(-8) + (5)(-14) + (1)(54)$$

$$= 0 \text{ ตั้งฉาก } \#$$